theories/interop/prims.v
@@ -1,0 +1,72 @@
+From Coq Require Import ssreflect.
+From stdpp Require Import base strings gmap.
+
+Inductive prim :=
+  | Palloc | Pregisterroot | Punregisterroot
+  | Pmodify | Preadfield | Pval2int | Pint2val.
+
+Inductive is_prim : string → prim → Prop :=
+  | alloc_is_prim : is_prim "alloc" Palloc
+  | registerroot_is_prim : is_prim "registerroot" Pregisterroot
+  | unregisterroot_is_prim : is_prim "unregisterroot" Punregisterroot
+  | modify_is_prim : is_prim "modify" Pmodify
+  | readfield_is_prim : is_prim "readfield" Preadfield
+  | val2int_is_prim : is_prim "val2int" Pval2int
+  | int2val_is_prim : is_prim "int2val" Pint2val.
+
+Global Hint Constructors is_prim : core.
+
+Ltac inv_is_prim :=
+  repeat match goal with
+  | H : is_prim (String _ _) _ |- _ => inversion H; subst; clear H
+  end.
+
+Lemma is_prim_inj s p1 p2 :
+  is_prim s p1 →
+  is_prim s p2 →
+  p1 = p2.
+Proof. inversion 1; inversion 1; by simplify_eq. Qed.
+
+Ltac is_prim_inj :=
+  repeat match goal with
+  | H1 : is_prim ?s ?p1, H2 : is_prim ?s ?p2 |- _ =>
+      pose proof (is_prim_inj _ _ _ H1 H2); subst p2; clear H2
+  end.
+
+Global Instance is_prim_dec s : Decision (∃ p, is_prim s p).
+Proof.
+  destruct (decide (s = "alloc")) as [->|]. left; eexists; constructor.
+  destruct (decide (s = "registerroot")) as [->|]. left; eexists; constructor.
+  destruct (decide (s = "unregisterroot")) as [->|]. left; eexists; constructor.
+  destruct (decide (s = "modify")) as [->|]. left; eexists; constructor.
+  destruct (decide (s = "readfield")) as [->|]. left; eexists; constructor.
+  destruct (decide (s = "val2int")) as [->|]. left; eexists; constructor.
+  destruct (decide (s = "int2val")) as [->|]. left; eexists; constructor.
+  right. by intros [? H]; inversion H.
+Qed.
+
+Definition prims_prog : gmap string prim :=
+  list_to_map [
+      ("alloc", Palloc);
+      ("registerroot", Pregisterroot);
+      ("unregisterroot", Punregisterroot);
+      ("modify", Pmodify);
+      ("readfield", Preadfield);
+      ("val2int", Pval2int);
+      ("int2val", Pint2val)
+  ].
+
+Lemma lookup_prims_prog s p :
+  prims_prog !! s = Some p ↔ is_prim s p.
+Proof.
+  rewrite /prims_prog /=. split.
+  { intros H.
+    destruct (decide (s = "alloc")) as [->|]; simplify_map_eq; first constructor.
+    destruct (decide (s = "registerroot")) as [->|]; simplify_map_eq; first constructor.
+    destruct (decide (s = "unregisterroot")) as [->|]; simplify_map_eq; first constructor.
+    destruct (decide (s = "modify")) as [->|]; simplify_map_eq; first constructor.
+    destruct (decide (s = "readfield")) as [->|]; simplify_map_eq; first constructor.
+    destruct (decide (s = "val2int")) as [->|]; simplify_map_eq; first constructor.
+    destruct (decide (s = "int2val")) as [->|]; simplify_map_eq; first constructor. }
+  { inversion 1; by simplify_map_eq. }
+Qed.
