theories/interop/wrapper_wp_ext_call_laws.v
@@ -11,7 +11,7 @@ From melocoton Require Import big_sepM_limited.
 From iris.proofmode Require Import proofmode.
 From melocoton.ml_toy_lang Require Import lang melocoton.lang_instantiation melocoton.primitive_laws.
 From melocoton.c_toy_lang Require Import lang melocoton.lang_instantiation melocoton.primitive_laws notation.
-From melocoton.interop Require Import linking_wp basics wrapper_wp wrapper_wp_block_sim wrapper_wp_utils.
+From melocoton.interop Require Import linking_wp basics prims wrapper_wp wrapper_wp_block_sim wrapper_wp_utils.
 Import Wrap.
 
 Section Laws.
@@ -98,6 +98,37 @@ Local Ltac SI_not_at_boundary :=
   iDestruct (SI_not_at_boundary_is_in_ML with "Hσ Hnb") as %(ρc & mem & ->);
   iNamed "Hσ"; iNamed "SIC".
 
+Lemma wp_pre_cases_c_prim T wp prm_name prm ρc mem E K ws Φ :
+  p !! prm_name = None →
+  is_prim prm_name prm →
+  (∃ w ρc' mem', c_prim_step prm ws ρc mem w ρc' mem') →
+  (∀ w ρc' mem',
+    ⌜c_prim_step prm ws ρc mem w ρc' mem'⌝ -∗
+    |={E}▷=> weakestpre.state_interp (CState ρc' mem') ∗ wp E (ExprC (language.fill K (C_lang.Val w))) Φ) -∗
+  wp_pre_cases (p : prog wrap_lang) T wp (CState ρc mem) E
+    (ExprC (c_toy_lang.melocoton.lang_instantiation.fill K (FunCall &prm_name (map Val ws))))
+    Φ.
+Proof.
+  iIntros (Hnp Hprm Hcstep) "HWP".
+  iRight. iRight. iSplit.
+  { iPureIntro. destruct Hcstep as (? & ? & ? & ?).
+    econstructor. eapply head_prim_step.
+    eapply (PrimS _ _ _ _ _ _ _ _ _ _ _ (λ _, True)); try done.
+    rewrite /language.to_call /= map_unmap_val //. }
+  { iIntros (X Hstep).
+    destruct Hstep as ([] & x & Hre & Hstep).
+    change (fill () x) with x in *. subst x.
+    cbn in Hstep; unfold step,mrel in Hstep; cbn in Hstep.
+    inversion Hstep; simplify_eq.
+    { exfalso. by eapply (call_no_StepCS ws). }
+    { exfalso. by eapply (call_no_RetS ws). }
+    { edestruct (call_inversion ws) as (? & ? & ?);
+        [apply Hnp | done | done | ..].
+      simplify_eq. unfold Wrap.fill in *. is_prim_inj.
+      iSpecialize ("HWP" with "[]"); first done.
+      iMod "HWP". do 2 iModIntro. iMod "HWP". iModIntro. eauto. } }
+Qed.
+
 Lemma wp_ext_call_int2val : ext_call_is_sound WP_int2val_spec.
 Proof.
   intros E T s vv K Ξ Φ.
@@ -105,23 +136,15 @@ Proof.
   iIntros "%Hnone Hnb HT IH %σ Hσ". cbn.
   SI_not_at_boundary. iNamed "HT".
   iNamed "HGC". SI_GC_agree.
-  iModIntro. iRight. iRight. iSplitR.
-  + iPureIntro. econstructor. eapply head_prim_step.
-    eapply (PrimInt2valS _ _ _ _ _ _ _ (fun k => True)).
-    2: econstructor. 2: done.
-    cbn. done.
-  + iIntros (X Hstep).
-    destruct Hstep as ([] & x & Hre & Hstep). change (fill () x) with x in Hre. subst x.
-    cbn in Hstep; unfold step,mrel in Hstep; cbn in Hstep.
-    inversion_call_step Hstep ([ #z]).
-    do 3 iModIntro.
-    do 2 iExists _. change (Wrap.fill () ?x) with (x) in *.
-    iSplit; first by eauto. simplify_eq.
-    iSplitL "SIζ SIχ SIθ SIroots SIbound HnC HσC".
-    { iFrame. eauto. }
-    iApply ("IH" with "[-Hnb] Hnb").
-    iApply ("HWP" with "[-]"); last done.
-    do 10 iExists _; rewrite /named; iFrame. eauto.
+  iModIntro. iApply wp_pre_cases_c_prim; [done|by eauto|..].
+  { do 3 eexists; constructor; eauto. }
+  iIntros (w ρc' mem' Hstep) "!> !> !>".
+  inversion Hstep; simplify_eq. inv_repr_lval.
+  iSplitL "SIζ SIχ SIθ SIroots SIbound HnC HσC".
+  { iFrame. eauto. }
+  iApply ("IH" with "[-Hnb] Hnb").
+  iApply ("HWP" with "[-]"); last done.
+  do 10 iExists _; rewrite /named; iFrame. eauto.
 Qed.
 
 Lemma wp_ext_call_val2int : ext_call_is_sound WP_val2int_spec.
@@ -130,20 +153,14 @@ Proof.
   rewrite weakestpre.wp_unfold. rewrite /weakestpre.wp_pre.
   iIntros "%Hnone Hnb HT IH %σ Hσ".
   SI_not_at_boundary. iNamed "HT". iNamed "HGC". SI_GC_agree.
-  iModIntro. iRight. iRight. iSplitR.
-  + iPureIntro. econstructor. eapply head_prim_step.
-    eapply (PrimVal2intS _ _ _ _ _ _ _ (fun k => True)). 2: apply Hrepr. all:done.
-  + iIntros (X Hstep).
-    destruct Hstep as ([] & x & Hre & Hstep). change (fill () x) with x in Hre. subst x.
-    cbn in Hstep; unfold step,mrel in Hstep; cbn in Hstep.
-    inversion_call_step Hstep ([w]).
-    do 3 iModIntro.
-    do 2 iExists _. change (Wrap.fill () ?x) with (x) in *.
-    iSplit; first by eauto. simplify_eq.
-    iSplitL "SIζ SIχ SIθ SIroots SIbound HnC HσC".
-    { iFrame; eauto. }
-    iApply ("IH" with "[-Hnb] Hnb").
-    inv_repr_lval. iApply ("HWP"). do 10 iExists _; unfold named; iFrame. eauto.
+  iModIntro. iApply wp_pre_cases_c_prim; [done|by eauto|..].
+  { do 3 eexists; constructor; eauto. }
+  iIntros (w' ρc' mem' Hstep) "!> !> !>".
+  inversion Hstep; subst. inv_repr_lval.
+  iSplitL "SIζ SIχ SIθ SIroots SIbound HnC HσC".
+  { iFrame; eauto. }
+  iApply ("IH" with "[-Hnb] Hnb").
+  iApply ("HWP"). do 10 iExists _; unfold named; iFrame. eauto.
 Qed.
 
 Lemma wp_ext_call_registerroot : ext_call_is_sound WP_registerroot_spec.
@@ -152,40 +169,30 @@ Proof.
   rewrite weakestpre.wp_unfold. rewrite /weakestpre.wp_pre.
   iIntros "%Hnone Hnb HT IH %σ Hσ".
   SI_not_at_boundary. iNamed "HT". iNamed "HGC". SI_GC_agree.
-
-  iAssert (⌜l ∈ dom roots_m⌝ → False)%I as "%Hdom".
+  iAssert (⌜¬ l ∈ dom roots_m⌝)%I as "%Hdom".
   1: { iIntros "%H". eapply elem_of_dom in H; destruct H as [k Hk].
        iPoseProof (big_sepM_lookup_acc with "GCrootspto") as "((%ww&Hww&_)&_)".
        1: apply Hk. iPoseProof (mapsto_ne with "Hpto Hww") as "%Hne". congruence. }
-
-  iModIntro. iRight. iRight. iSplitR.
-  + iPureIntro. econstructor. eapply head_prim_step.
-    eapply (PrimRegisterrootS _ _ _ _ _ _ _ (fun k => True)). 1,3,4: done.
-    intros H; apply Hdom; congruence.
-  + iIntros (X Hstep).
-    destruct Hstep as ([] & x & Hre & Hstep). change (fill () x) with x in Hre. subst x.
-    cbn in Hstep; unfold step,mrel in Hstep; cbn in Hstep.
-    inversion_call_step Hstep ([ #l ]). subst.
-
-    iMod (ghost_var_update_halves with "SIroots GCroots") as "(SIroots&GCroots)".
-    iMod (ghost_map_insert with "GCrootsm") as "(GCrootsm&Hres)".
-    1: eapply not_elem_of_dom; intros Hc; eapply Hdom; done.
-    iPoseProof (big_sepM_insert) as "(_&HR)".
-    1: eapply not_elem_of_dom; intros Hc; eapply Hdom; done.
-    iPoseProof ("HR" with "[Hpto GCrootspto]") as "GCrootspto"; first iFrame "GCrootspto".
-    iExists w; iFrame; done.
-    iClear "HR".
-    do 3 iModIntro.
-    do 2 iExists _. change (Wrap.fill () ?x) with (x) in *.
-    iSplit; first by eauto.
-    iSplitL "SIζ SIχ SIθ SIroots SIbound HnC HσC".
-    { iFrame; eauto. }
-    iApply ("IH" with "[-Hnb] Hnb").
-    iApply ("HWP" with "[-Hres] Hres").
-    do 10 iExists _. unfold named. iFrame. iPureIntro; split_and!; eauto.
-    - rewrite dom_insert_L. rewrite (_: dom roots_m = rootsC ρc) //.
-    - intros ℓ γ [[-> ->]|[Hne HH]]%lookup_insert_Some; last by eapply Hrootslive.
-      inv_repr_lval. by eapply elem_of_dom_2.
+  iModIntro. iApply wp_pre_cases_c_prim; [done|by eauto|..].
+  { do 3 eexists; constructor; eauto. set_solver. }
+  iIntros (w' ρc' mem' Hstep) "!> !>".
+  inversion Hstep; subst.
+  iMod (ghost_var_update_halves with "SIroots GCroots") as "(SIroots&GCroots)".
+  iMod (ghost_map_insert with "GCrootsm") as "(GCrootsm&Hres)".
+  1: eapply not_elem_of_dom; intros Hc; eapply Hdom; done.
+  iPoseProof (big_sepM_insert) as "(_&HR)".
+  1: eapply not_elem_of_dom; intros Hc; eapply Hdom; done.
+  iPoseProof ("HR" with "[Hpto GCrootspto]") as "GCrootspto"; first iFrame "GCrootspto".
+  iExists w; iFrame; done.
+  iClear "HR". iModIntro.
+  iSplitL "SIζ SIχ SIθ SIroots SIbound HnC HσC".
+  { iFrame; eauto. }
+  iApply ("IH" with "[-Hnb] Hnb").
+  iApply ("HWP" with "[-Hres] Hres").
+  do 10 iExists _. unfold named. iFrame. iPureIntro; split_and!; eauto.
+  - rewrite dom_insert_L. rewrite (_: dom roots_m = rootsC ρc) //.
+  - intros ℓ γ [[-> ->]|[Hne HH]]%lookup_insert_Some; last by eapply Hrootslive.
+    inv_repr_lval. by eapply elem_of_dom_2.
 Qed.
 
 Lemma wp_ext_call_unregisterroot : ext_call_is_sound WP_unregisterroot_spec.
@@ -195,31 +202,22 @@ Proof.
   iIntros "%Hnone Hnb HT IH %σ Hσ".
   SI_not_at_boundary. iNamed "HT". iNamed "HGC". SI_GC_agree.
   iPoseProof (ghost_map_lookup with "GCrootsm Hpto") as "%Helem".
-
-  iModIntro. iRight. iRight. iSplitR.
-  + iPureIntro. econstructor. eapply head_prim_step.
-    eapply (PrimUnregisterrootS _ _ _ _ _ _ _ (fun k => True)). 1,3,4: done.
-    rewrite (_: rootsC ρc = dom roots_m) //. by eapply elem_of_dom_2.
-  + iIntros (X Hstep).
-    destruct Hstep as ([] & x & Hre & Hstep). change (fill () x) with x in Hre. subst x.
-    cbn in Hstep; unfold step,mrel in Hstep; cbn in Hstep.
-    inversion_call_step Hstep ([ #l ]). subst.
-
-    iMod (ghost_var_update_halves with "SIroots GCroots") as "(SIroots&GCroots)".
-    iMod (ghost_map_delete with "GCrootsm Hpto") as "GCrootsm".
-    iPoseProof (big_sepM_delete) as "(HL&_)"; first eapply Helem.
-    iPoseProof ("HL" with "GCrootspto") as "((%W&Hpto&%Hw)&GCrootspto)".
-    iClear "HL".
-    do 3 iModIntro.
-    do 2 iExists _. change (Wrap.fill () ?x) with (x) in *.
-    iSplit; first by eauto.
-    iSplitL "SIζ SIχ SIθ SIroots SIbound HnC HσC".
-    { iFrame; eauto. }
-    iApply ("IH" with "[-Hnb] Hnb").
-    iApply ("HWP" $! W with "[-Hpto] Hpto []"). 2: done.
-    do 10 iExists _. iFrame. iPureIntro; split_and!; eauto.
-    - rewrite dom_delete_L. rewrite (_: dom roots_m = rootsC ρc) //.
-    - intros ℓ γ [HH1 HH2]%lookup_delete_Some; by eapply Hrootslive.
+  iModIntro. iApply wp_pre_cases_c_prim; [done|by eauto|..].
+  { do 3 eexists; constructor; eauto.
+    rewrite (_: rootsC ρc = dom roots_m) //. by eapply elem_of_dom_2. }
+  iIntros (w' ρc' mem' Hstep) "!> !>". inversion Hstep; subst.
+  iMod (ghost_var_update_halves with "SIroots GCroots") as "(SIroots&GCroots)".
+  iMod (ghost_map_delete with "GCrootsm Hpto") as "GCrootsm".
+  iPoseProof (big_sepM_delete) as "(HL&_)"; first eapply Helem.
+  iPoseProof ("HL" with "GCrootspto") as "((%W&Hpto&%Hw)&GCrootspto)".
+  iClear "HL". iModIntro.
+  iSplitL "SIζ SIχ SIθ SIroots SIbound HnC HσC".
+  { iFrame; eauto. }
+  iApply ("IH" with "[-Hnb] Hnb").
+  iApply ("HWP" $! W with "[-Hpto] Hpto []"). 2: done.
+  do 10 iExists _. iFrame. iPureIntro; split_and!; eauto.
+  - rewrite dom_delete_L. rewrite (_: dom roots_m = rootsC ρc) //.
+  - intros ℓ γ [HH1 HH2]%lookup_delete_Some; by eapply Hrootslive.
 Qed.
 
 Lemma wp_ext_call_modify : ext_call_is_sound WP_modify_spec.
@@ -234,61 +232,50 @@ Proof.
        destruct Hfreezeρ as [HL HR].
        assert (γ ∈ dom (ζC ρc)) as [v Hv]%elem_of_dom by by (rewrite HL; eapply elem_of_dom_2).
        specialize (HR _ _ _ Hv Helem) as Hinv. inversion Hinv; subst; done. }
-
-  iModIntro. iRight. iRight. iSplitR.
-  + iPureIntro. econstructor. eapply head_prim_step.
-    eapply (PrimModifyS _ _ _ _ _ _ _ _ _ _ _ _ _ (fun k => True)); try done.
-    eapply mk_modify_block. lia.
-  + iIntros (X Hstep).
-    destruct Hstep as ([] & x & Hre & Hstep). change (fill () x) with x in Hre. subst x.
-    cbn in Hstep; unfold step,mrel in Hstep; cbn in Hstep.
-    inversion_call_step Hstep ([ w; #i; w' ]). subst.
-    iMod (lstore_own_update _ _ _ _ blk' with "GCζvirt Hpto") as "(GCζvirt&Hpto)".
-    iMod (ghost_var_update_halves with "SIζ GCζ") as "(SIζ&GCζ)".
-    iPoseProof (interp_ML_discarded_locs_pub with "GCσMLv GCχNone") as "%Hpublocs".
-
-    do 3 iModIntro.
-    do 2 iExists _. change (Wrap.fill () ?x) with (x) in *.
-    inv_repr_lval.
-    destruct HGCOK as [HGCL HGCR]. exploit_gmap_inj. repr_lval_inj.
-    iSplit; first by eauto.
-    iSplitL "SIζ SIχ SIθ SIroots SIbound HnC HσC".
-    { iFrame; eauto. }
-
-    iApply ("IH" with "[-Hnb] Hnb").
-    change (Z.of_nat 0) with (Z0).
-    iApply ("HWP" with "[-Hpto] [Hpto]").
-    { iExists _, (<[γ:=blk']> (ζσ ∪ ζvirt)), ζσ, (<[γ:=blk']>ζvirt), _, χvirt, σMLvirt.
-      iExists _, _, _. unfold named. iFrame.
-      erewrite pub_locs_in_lstore_insert_existing; last by eapply elem_of_dom_2. iFrame.
-      iPureIntro; split_and!; eauto; cbn. 1: destruct Hfreezeρ as [HL HR]; split.
-      - by erewrite !dom_insert_L, HL.
-      - intros γ' b1 b2 [[? ?]|[Hne1 H1]]%lookup_insert_Some [[??]|[Hne2 H2']]%lookup_insert_Some; try congruence.
-        1: subst; econstructor.
-        subst. by eapply HR.
-      - rewrite insert_union_r; first done.
-        erewrite map_disjoint_Some_l; done.
-      - eapply map_disjoint_dom. erewrite dom_insert_lookup; last by eexists. by eapply map_disjoint_dom.
-      - rewrite dom_insert_lookup; last by eexists. 
-        done.
-      - intros ℓ Vs γ1 bb H1 H2' [[<- <-]|[Hne H3']]%lookup_insert_Some.
-        -- epose proof (map_Forall_lookup_1 _ _ γ ℓ Hpublocs) as Hpub2. cbn in Hpub2.
-           rewrite Hpub2 in H1; first congruence.
-           eapply pub_locs_in_lstore_lookup; last apply H2'.
-           eapply elem_of_dom_2; done.
-        -- specialize (Hstore _ _ _ _ H1 H2' H3'); inversion Hstore; subst.
-           econstructor. eapply Forall2_impl; first done.
-           intros x' y HH; eapply is_val_insert_immut; last done.
-           1: erewrite lookup_union_r; first done.
-           1: eapply map_disjoint_Some_l; done. done.
-      - split; first apply HGCL.
-        intros γ0 m1 tg1 vs1 γ1 Hγ0 [[??]|[Hne1 Hlu]]%lookup_insert_Some Hlloc.
-        2: by eapply HGCR. simplify_eq. inv_modify_block.
-        apply list_insert_lookup_inv in Hlloc as [HLL|HRR]; simplify_map_eq.
-        { inv_repr_lval. by eapply elem_of_dom_2. }
-        { eapply HGCR; eauto. rewrite lookup_union_r //.
-          eapply map_disjoint_Some_l; eauto. } }
-    { iSplit. inv_modify_block; simplify_map_eq. iFrame. eauto. }
+  iModIntro. iApply wp_pre_cases_c_prim; [done|by eauto|..].
+  { do 3 eexists. econstructor; eauto. econstructor. lia. }
+  iIntros (w'' ρc' mem' Hstep) "!> !>". inversion Hstep; subst. inv_repr_lval.
+  destruct HGCOK as [HGCL HGCR]. exploit_gmap_inj. repr_lval_inj.
+  iMod (lstore_own_update _ _ _ _ blk' with "GCζvirt Hpto") as "(GCζvirt&Hpto)".
+  iMod (ghost_var_update_halves with "SIζ GCζ") as "(SIζ&GCζ)".
+  iPoseProof (interp_ML_discarded_locs_pub with "GCσMLv GCχNone") as "%Hpublocs".
+  iModIntro.
+  iSplitL "SIζ SIχ SIθ SIroots SIbound HnC HσC".
+  { iFrame; eauto. }
+  iApply ("IH" with "[-Hnb] Hnb").
+  change (Z.of_nat 0) with (Z0).
+  iApply ("HWP" with "[-Hpto] [Hpto]").
+  { iExists _, (<[γ:=blk']> (ζσ ∪ ζvirt)), ζσ, (<[γ:=blk']>ζvirt), _, χvirt, σMLvirt.
+    iExists _, _, _. unfold named. iFrame.
+    erewrite pub_locs_in_lstore_insert_existing; last by eapply elem_of_dom_2. iFrame.
+    iPureIntro; split_and!; eauto; cbn. 1: destruct Hfreezeρ as [HL HR]; split.
+    - by erewrite !dom_insert_L, HL.
+    - intros γ' b1 b2 [[? ?]|[Hne1 H1']]%lookup_insert_Some [[??]|[Hne2 H2']]%lookup_insert_Some; try congruence.
+      1: subst; econstructor.
+      subst. by eapply HR.
+    - rewrite insert_union_r; first done.
+      erewrite map_disjoint_Some_l; done.
+    - eapply map_disjoint_dom. erewrite dom_insert_lookup; last by eexists. by eapply map_disjoint_dom.
+    - rewrite dom_insert_lookup; last by eexists.
+      done.
+    - intros ℓ Vs γ1 bb H1' H2' [[<- <-]|[Hne H3']]%lookup_insert_Some.
+      -- epose proof (map_Forall_lookup_1 _ _ γ ℓ Hpublocs) as Hpub2. cbn in Hpub2.
+         rewrite Hpub2 in H1'; first congruence.
+         eapply pub_locs_in_lstore_lookup; last apply H2'.
+         eapply elem_of_dom_2; done.
+      -- specialize (Hstore _ _ _ _ H1' H2' H3'); inversion Hstore; subst.
+         econstructor. eapply Forall2_impl; first done.
+         intros x' y HH; eapply is_val_insert_immut; last done.
+         1: erewrite lookup_union_r; first done.
+         1: eapply map_disjoint_Some_l; done. done.
+    - split; first apply HGCL.
+      intros γ0 m1 tg1 vs1 γ1 Hγ0 [[??]|[Hne1 Hlu]]%lookup_insert_Some Hlloc.
+      2: by eapply HGCR. simplify_eq. inv_modify_block.
+      apply list_insert_lookup_inv in Hlloc as [HLL|HRR]; simplify_map_eq.
+      { inv_repr_lval. by eapply elem_of_dom_2. }
+      { eapply HGCR; eauto. rewrite lookup_union_r //.
+        eapply map_disjoint_Some_l; eauto. } }
+  { iSplit. inv_modify_block; simplify_map_eq. iFrame. eauto. }
 Qed.
 
 Lemma wp_ext_call_readfield : ext_call_is_sound WP_readfield_spec.
@@ -316,26 +303,17 @@ Proof.
        erewrite lookup_union_r; first done.
        eapply map_disjoint_Some_l; done. }
 
-  iModIntro. iRight. iRight. iSplitR.
-  + iPureIntro. econstructor. eapply head_prim_step.
-    eapply (PrimReadfieldS _ _ _ _ _ _ _ _ _ _ _ _ _ (fun k => True)); eauto.
-  + iIntros (X Hstep).
-    destruct Hstep as ([] & x & Hre & Hstep). change (fill () x) with x in Hre. subst x.
-    cbn in Hstep; unfold step,mrel in Hstep; cbn in Hstep.
-    inversion_call_step Hstep ([ #a ; #i ]). subst.
-    inv_repr_lval. exploit_gmap_inj. simplify_map_eq.
-
-    do 3 iModIntro.
-    do 2 iExists _. change (Wrap.fill () ?x) with (x) in *.
-    iSplit; first by eauto.
-
-    iSplitL "SIζ SIχ SIθ SIroots SIbound HnC HσC".
-    { iFrame; eauto. }
-    iApply ("IH" with "[-Hnb] Hnb").
-    iApply ("HWP" with "[-Hpto] [Hpto] [] []"); try done.
-    rewrite /GC /named.
-    iExists _, (ζσ ∪ ζvirt), ζσ, ζvirt, _, χvirt, σMLvirt, _. iExists _, _.
-    iFrame. iPureIntro; split_and!; eauto. done.
+  iModIntro. iApply wp_pre_cases_c_prim; [done|by eauto|..].
+  { do 3 eexists; econstructor; eauto. }
+  iIntros (w'' ρc' mem' Hstep) "!> !> !>". inversion Hstep.
+  inv_repr_lval. exploit_gmap_inj. simplify_eq.
+  iSplitL "SIζ SIχ SIθ SIroots SIbound HnC HσC".
+  { iFrame; eauto. }
+  iApply ("IH" with "[-Hnb] Hnb").
+  iApply ("HWP" with "[-Hpto] [Hpto] [] []"); try done.
+  rewrite /GC /named.
+  iExists _, (ζσ ∪ ζvirt), ζσ, ζvirt, _, χvirt, σMLvirt, _. iExists _, _.
+  iFrame. iPureIntro; split_and!; eauto. done.
 Qed.
 
 Ltac solve_ext_call H := 
@@ -350,10 +328,7 @@ Proof.
   intros E T s vv K Ξ Φ.
   rewrite weakestpre.wp_unfold. rewrite /weakestpre.wp_pre.
   iIntros "%Hnone Hnb HT IH %σ Hσ".
-  destruct σ as [ρml σ | ρc mem].
-  1: iExFalso; iNamed "Hσ"; iNamed "SIML"; iPoseProof (ghost_var_agree with "Hnb SIbound") as "%HH"; congruence.
-  iNamed "Hσ"; iNamed "SIC".
-  cbn. iDestruct "HT" as "[H|[H|[H|[H|[H|H]]]]]".
+  SI_not_at_boundary. cbn. iDestruct "HT" as "[H|[H|[H|[H|[H|H]]]]]".
   - solve_ext_call wp_ext_call_int2val.
   - solve_ext_call wp_ext_call_val2int.
   - solve_ext_call wp_ext_call_registerroot.
@@ -362,6 +337,5 @@ Proof.
   - solve_ext_call wp_ext_call_readfield.
   (* - solve_ext_call wp_ext_call_alloc. *)
 Qed.
-
 
 End Laws.
